
\input{./src/preamble.tex}

\begin{document}

\title{Study of a predator prey model.}
\author{Moritz Wolter}

\maketitle

\section{The equation}
\begin{align}
\dot{x} &= x(x-a)(1-x) - bxy \\
\dot{y} &= xy - cy - d.
\label{eq:toBeAn}
\end{align}
With $a = 0.4, \; b = 0.3, \text{ and } c \in [0.65 0.75]$. $x$ represents prey and $y$ predators. The $xy$ products of the system govern the interaction of the two species. 

\section{Analysis of a simplified model $d=0$}
\subsection{One-dimensional approach}
Setting d and y equal to zero turns the system into:
\begin{equation}
\dot{x} = x(x-a)(1-x).
\label{eq:simple}
\end{equation}
For this simplified case the fixed points may be read off easily. $\dot{x} = 0$ yields $x_1 = 0, \; x_2 = a, \; x_3 = 1$. Linear analysis will lead to further insight into the nature of these fixed points reading of $f(x) =  x(x-a)(1-x)$ and computing $f'(x)$ leads to:
\begin{equation}
f'(x) = -3x^2 + 2x + 2xa -a.
\end{equation}
Substituting x with the fixed points yields:
\begin{align}
f'(x_1) &= -a \\
f'(x_2) &= -a^2 +a = -0.4^2 + 0.4 > 0 \\
f'(x_3) &= -3 + 2 + 2a - a = -1 + a = -0.6 < 0 
\end{align}
Thus it may be concluded, that $x_2$ is unstable and $x_3 \wedge x_1$ are stable.  
\begin{figure}
\centering
\input{./plots/simpleSim.tex}
\caption{Simulation of the simplified system described by equation~\ref{eq:simple}.}
\label{fig:simpleSim}
\end{figure}
Figure~\ref{fig:simpleSim} shows simulation results produced by a Runge-Kutta type numerical integration routine. The fixed point positions that where read off from the simplified system equation are confirmed by the results to be at $x_1 = 0, \; x_2 = a = 0.4, \; x_3 = 1$. Furthermore the fixed points show the predicted characteristics.

\subsection{Two-dimensional approach}
Once more the analysis starts with the computation of the fixed point locations. Setting the system equations to zero leads to:
\begin{align}
0 &= x(x-a)(1-x) - bxy \\
\label{eq:topDzero}
0 &= xy - cy.
\end{align}
Starting from the top equation~\ref{eq:topDzero} first x may be factored out:
\begin{equation}
0 = x[(x-a)(1-x) - by].
\end{equation}
Therefore $x_1 = 0$. In order to obtain the remaining zeros the equation:
\begin{align}
0 = (x - a)(1 - x) - by
\end{align} 
has to be solved. After factoring out the brackets the pq-Formula is applicable thus the following expression is obtained:
\begin{equation}
x_{2,3} = \frac{1+a}{2} \pm \sqrt{\frac{(1+a)^2}{4} - (a + by)}.
\label{eq:pq}
\end{equation}
Which will be simplified further once more is known about y. To finish the quest for the fixed points x values y is factored out in the second equation:
\begin{equation}
0 = y (x - c).
\label{eq:facDzero}
\end{equation}
The equation~\ref{eq:facDzero} is zero when $x_4 = c$. Which is the missing x component. Looking at y, $y_1 = 0$ is quickly read off from ~\ref{eq:facDzero}. Turning back to equation~\ref{eq:topDzero} and solving for $y$ while assuming $x \ne 0$ gives:
\begin{equation}
y_2 = \frac{(x - a)(1 - x)}{b}
\end{equation}
At this point two steady state solutions at $\begin{pmatrix} x_1 & y_1 \end{pmatrix}^T = \begin{pmatrix} 0 & 0 \end{pmatrix}^T$ and $\begin{pmatrix} x_4 & y_2 \end{pmatrix}^T = \begin{pmatrix} c & \frac{(c -a )(1-c)}{b} \end{pmatrix}^T$ are already known. Using $y_1$ again equation \ref{eq:pq} can be simplified further after plugging in and factoring out one obtains:
\begin{align}
x_{2/3} = \frac{1+a}{2} \pm \sqrt{\frac{1 - 2a + a^2}{4} } \\
x_{2/3} = \frac{1+a}{2} \pm \sqrt{(\frac{1 - a}{2})^2 } \\
x_{2/3} = \frac{1+a}{2} \pm \frac{1 - a}{2} \\
\Rightarrow x_2 = 1 \wedge x_3 = a
\end{align}
Now two more fixed points are known $\begin{pmatrix} x_2 & y_1 \end{pmatrix}^T = \begin{pmatrix} 1 & 0 \end{pmatrix}^T$ and 
$\begin{pmatrix} x_3 & y_1 \end{pmatrix}^T = \begin{pmatrix} a & 0 \end{pmatrix}^T$. 

\begin{table}
\centering
\begin{tabular}{|c|}
\hline
$\mathbf{x}_1^* = \begin{pmatrix} x_1 \\ y_1 \end{pmatrix} = \begin{pmatrix} 0 \\ 0 \end{pmatrix}$ \\
\hline
$\mathbf{x}_2^* =\begin{pmatrix} x_4 \\ y_2 \end{pmatrix} = \begin{pmatrix} c \\ \frac{(c -a )(1-c)}{b} \end{pmatrix}$\\
\hline
$\mathbf{x}_3^* =\begin{pmatrix} x_2 \\ y_1 \end{pmatrix} = \begin{pmatrix} 1 \\ 0 \end{pmatrix}$\\
\hline
$\mathbf{x}_4^* =\begin{pmatrix} x_3 \\ y_1 \end{pmatrix} = \begin{pmatrix} a \\ 0 \end{pmatrix}$\\
\hline
\end{tabular}
\caption{Fixed point positions.}
\end{table}

Next the obtained points will be classified according to their properties. Starting from the system equations after factoring out the Jacobian is computed:
\begin{equation}
J = \begin{pmatrix}
-3x^2 + 2x + 2xa - a - yb & - bx \\
y & x-c \\
\end{pmatrix}
\end{equation}
Linear analysis proceeds by plugging the fixed points into the Jacobian and compute the trace $\tau$ as well as the determinant $\triangle$. For the first fixed point $\mathbf{x}_1^*$ this gives:
\begin{equation}
J(\mathbf{x}_1^*) = \begin{pmatrix}
-a & 0 \\
0  & -c \end{pmatrix}.
\end{equation}
Therefore the trace and determinant are $\tau_1 = -a-c \wedge \triangle_1 = ac$. Thus this node is a saddle point if $c < 0$, if $c > 0$ it is stable if $-a < c$ and spirals if $a < c$.
The second fixed point $\mathbf{x}_2^*$ has the Jacobian:
\begin{equation}
J(\mathbf{x_2^*}) = \begin{pmatrix}
c(c+a-2c) & - bc \\
(c-a)(1-c)/b &	0
\end{pmatrix})
\end{equation}
With the determinant and trace $\tau_2 = c(1+a-2c) \wedge \triangle_2 = c(c-a)(1-c)$. From these two expressions it is possible to deduce, that if $c>0$, $\mathbf{x_2^*}$ is a saddle point if additionally, $c > a \wedge c < 1$. If that is not the case then the determinant is positive, now the trace determines stability. $\tau_2 < 0$ is the case if $\frac{1+a}{2} < c$. However it $c < 0$ then the determinant will always be negative, making $\mathbf{x_2^*}$ a saddle point.















\end{document}